src/Dflatmajor.v
@@ -111,7 +111,7 @@ Inductive state: Type :=
              (stack: Z),                (**r current number of stack frames alloc *)
       state
   | Callstate:                  (**r Invocation of a function *)
-      forall (f: fundef)                (**r function to invoke *)
+      forall (f: function)                (**r function to invoke *)
              (args: list val)           (**r arguments provided by caller *)
              (k: cont)                  (**r what to do next  *)
              (m: mem)                   (**r memory state *)
@@ -210,7 +210,7 @@ Inductive step: state -> trace -> state -> Prop :=
   | step_call: forall f optid sig a bl k sp e m vfp vargs fd z,
       eval_expr e m sp a vfp ->
       eval_exprlist e m sp bl vargs ->
-      Genv.find_funct ge vfp = Some fd ->
+      Genv.find_funct ge vfp = Some (Internal fd) ->
       funsig fd = sig ->
       step (State f (Scall optid sig a bl) k sp e m z)
         E0 (Callstate fd vargs (Kcall optid f sp e k) m z)
@@ -266,7 +266,7 @@ Inductive initial_state (p: program): state -> Prop :=
       let ge := Genv.globalenv p in
       Genv.init_mem p = Some m0 ->
       Genv.find_symbol ge p.(prog_main) = Some b ->
-      Genv.find_funct_ptr ge b = Some f ->
+      Genv.find_funct_ptr ge b = Some (Internal f) ->
       funsig f = signature_main ->
       initial_state p (Callstate f nil Kstop m0 0).
 
